wip

DesugarScopedVarsProof.dfy
@@ -55,345 +55,323 @@ module DesugarScopedVarsProof {
     && m.Values !! s2Orig.Keys
   }
 
-  lemma RelStateLarger<V>(m: map<var_name, var_name>, m': map<var_name, var_name>, s1: map<var_name, V>, s2: map<var_name, V>, s2Orig: map<var_name, Option<V>>)
-  requires RelState2(m', s1, s2, s2Orig)
-  requires MapGte(m', m)
-  ensures RelState2(m, s1, s2, s2Orig)
-  {
-    reveal MapGte();
-    reveal RelState2();
-  }
-
   predicate {:opaque} RelPred<A(!new)>(m: map<var_name, var_name>, post1: Predicate<A>, post2: Predicate<A>, s2Orig: MapOrig<Val<A>>)
   {
     forall s, s' | RelState2(m, s, s', s2Orig) :: post1(s) == post2(s')
   }
 
-  predicate {:opaque} MapGte(m': map<var_name, var_name>, m: map<var_name, var_name>)
-  {
-    forall x | x in m.Keys :: x in m'.Keys && m[x] == m'[x]
-  }
-
- lemma RelState2UpdPreserve<V>(varMapping: map<var_name, var_name>, s1: map<var_name, V>, s2: map<var_name, V>, s2Orig: MapOrig<V>, x: var_name, v: V)
- requires RelState2(varMapping, s1, s2, s2Orig)
- requires Maps.Injective(varMapping)
- requires x in varMapping.Keys
- ensures RelState2(varMapping, s1[x := v], s2[varMapping[x] := v], s2Orig)
- {
-  reveal RelState2();
-  var x' := varMapping[x];
-  forall k | k in varMapping.Keys 
-  ensures Maps.Get(s1[x := v], k) == Maps.Get(s2[varMapping[x] := v], varMapping[k])
-  {
-    var k' := varMapping[k];
-    if k != x {
-      calc {
-        Maps.Get(s1[x := v], k);
-        Maps.Get(s1, k);
-        Maps.Get(s2, k');
-        { reveal Maps.Injective(); }
-        Maps.Get(s2[x' := v], k');
-      }
-    }
-  }
- }
-
- lemma RelState2UpdVarDeclsPreserve<A>(
-    varMapping: map<var_name, var_name>, 
-    s1: state<A>,
-    s2: state<A>, 
-    s2Orig: MapOrig<Val<A>>, 
-    varDecls: seq<VarDecl>, 
-    varDecls': seq<VarDecl>,
-    vs: seq<Val<A>>)
- requires RelState2(varMapping, s1, s2, s2Orig)
- requires Maps.Injective(varMapping)
- requires GetVarNames(varDecls) <= varMapping.Keys
- requires |vs| == |varDecls| == |varDecls'|
- requires (forall i | 0 <= i < |varDecls| :: varDecls'[i].0 == varMapping[varDecls[i].0])
- ensures RelState2(varMapping, StateUpdVarDecls(s1, varDecls, vs), StateUpdVarDecls(s2, varDecls', vs), s2Orig)
- {
-   if |varDecls| > 0 {       
-      var s1' := StateUpdVarDecls(s1, varDecls[1..], vs[1..]);
-      var s2' := StateUpdVarDecls(s2, varDecls'[1..], vs[1..]);
-
-      assert RelState2(varMapping, s1', s2', s2Orig) by {
-        RelState2UpdVarDeclsPreserve(varMapping, s1, s2, s2Orig, varDecls[1..], varDecls'[1..], vs[1..]);
-      }
-
-      RelState2UpdPreserve(varMapping, s1', s2', s2Orig, varDecls[0].0, vs[0]);
-   }
- }
-
- lemma ConvertRelState<V>(m: map<var_name, var_name>, s1: map<var_name, V>, s2: map<var_name, V>, s2Orig: MapOrig<V>)
- requires RelState2(m, s1, s2, s2Orig)
- ensures RelState(m, s1, s2)
- {
-  reveal RelState2();
-  reveal RelState();
- }
-
- lemma ForallVarDeclsRelNew<A(!new)>(
-    a: absval_interp<A>, 
-    varDecls: seq<(var_name, Ty)>, 
-    varMapping: map<var_name, var_name>, 
-    p1: Predicate<A>,
-    p2: Predicate<A>,
-    s2Orig: MapOrig<Val<A>>)
-    requires RelPred(varMapping, p1, p2, s2Orig)
-    requires GetVarNames(varDecls) <= varMapping.Keys
-    requires Maps.Injective(varMapping)
-    ensures 
-      var f := (vDecl : (var_name, Ty)) => 
-          if vDecl.0 in varMapping.Keys then (varMapping[vDecl.0], vDecl.1) else vDecl;
-      var varDecls' := Sequences.Map(f, varDecls);
-      RelPred(varMapping, ForallVarDeclsShallow(a, varDecls, p1), ForallVarDeclsShallow(a, varDecls', p2), s2Orig)
-  {
-    var f := (vDecl : (var_name, Ty)) => 
-        if vDecl.0 in varMapping.Keys then (varMapping[vDecl.0], vDecl.1) else vDecl;
-    var varDecls' := Sequences.Map(f, varDecls);
-    if |varDecls| == 0 {
-      //trivial
-      reveal ForallVarDeclsShallow();
-      assert ForallVarDeclsShallow(a, varDecls, p1) == p1;
-    } else {
-      var (x,t) := varDecls[0];
-      var x' := varMapping[x];
-
-      var f := (vDecl : (var_name, Ty)) => 
-          if vDecl.0 in varMapping.Keys then (varMapping[vDecl.0], vDecl.1) else vDecl;
-      var varDecls' := Sequences.Map(f, varDecls);
-
-      forall s1, s2 | RelState2(varMapping, s1, s2, s2Orig)
-      ensures ForallVarDeclsShallow(a, varDecls, p1)(s1) == ForallVarDeclsShallow(a, varDecls', p2)(s2)
-      {
-        forall vs | ValuesRespectDecls(a, vs, varDecls)
-        ensures p1(StateUpdVarDecls(s1, varDecls, vs)) == p2(StateUpdVarDecls(s2, varDecls', vs))
-        {
-          var s1' := StateUpdVarDecls(s1, varDecls, vs);
-          var s2' := StateUpdVarDecls(s2, varDecls', vs);
-          assert RelState2(varMapping, s1', s2', s2Orig) by {
-            RelState2UpdVarDeclsPreserve(varMapping, s1, s2, s2Orig, varDecls, varDecls', vs);
-          }
-          reveal RelPred();
-        }
-        ForallVarDeclsShallowEquiv(a, varDecls, varDecls', p1, p2, s1, s2);
-      }
-
-      reveal RelPred();
-    }
-  }
- lemma ForallVarDeclsRelNew2<A(!new)>(
-    a: absval_interp<A>, 
-    varDecls: seq<(var_name, Ty)>, 
-    varMapping: map<var_name, var_name>, 
-    p1: Predicate<A>,
-    p2: Predicate<A>,
-    s1: state<A>,
-    s2: state<A>,
-    sOrig: MapOrig<Val<A>>)
-    requires RelPred(varMapping, p1, p2, sOrig)
-    requires RelState2(varMapping, s1, s2, sOrig)
-    requires GetVarNames(varDecls) <= varMapping.Keys
-    requires Maps.Injective(varMapping)
-    ensures 
-      var f := (vDecl : (var_name, Ty)) => 
-          if vDecl.0 in varMapping.Keys then (varMapping[vDecl.0], vDecl.1) else vDecl;
-      var varDecls' := Sequences.Map(f, varDecls);
-      ForallVarDeclsShallow(a, varDecls, p1)(s1) ==  ForallVarDeclsShallow(a, varDecls', p2)(s2)
-  {
-    ForallVarDeclsRelNew(a, varDecls, varMapping, p1, p2, sOrig);
-    reveal RelPred();
-  }
-
- lemma {:induction false} SubstSimpleCmdCorrect<A(!new)>(a: absval_interp<A>, sc: SimpleCmd, varMapping: map<var_name, var_name>, 
-    post1: Predicate<A>, post2: Predicate<A>, s2Orig: MapOrig<Val<A>>)
-    requires RelPred(varMapping, post1, post2, s2Orig)
-    requires sc.WellFormedVars(varMapping.Keys)
-    requires Maps.Injective(varMapping)
-    ensures 
-      var sc' := SubstSimpleCmd(sc, varMapping);
-      RelPred(varMapping, WpShallowSimpleCmd(a, sc, post1), WpShallowSimpleCmd(a, sc', post2), s2Orig)
-  {
-    var sc' := SubstSimpleCmd(sc, varMapping);
-    var pre1 := WpShallowSimpleCmd(a, sc, post1);
-    var pre2 := WpShallowSimpleCmd(a, sc', post2);
-    forall s1:map<var_name, Val<A>>, s2 | RelState2(varMapping, s1, s2, s2Orig)
-      ensures pre1(s1) == pre2(s2)
-    {
-      ConvertRelState(varMapping, s1, s2, s2Orig);
-      reveal RelPred();
-      match sc {
-        case Skip => 
-        case Assume(e) => 
-          MultiSubstExprSpec2(a, varMapping, e, s1, s2);
-        case Assert(e) => 
-          reveal RelPred();
-          MultiSubstExprSpec2(a, varMapping, e, s1, s2);
-        case Assign(x, t, e) =>
-          var e' := MultiSubstExpr(e, varMapping);
-          var v1Opt := EvalExpr(a, e, s1);
-          var v2Opt := EvalExpr(a, e', s2);
-          assert v1Opt == v2Opt by {
-            reveal RelState();
-            reveal RelState2();
-            MultiSubstExprSpec2(a, varMapping, e, s1, s2);
-          }
-
-          if(v1Opt.Some?) {
-            var v := v1Opt.value;
-            var x' := varMapping[x];
-
-            assert RelState2(varMapping, s1[x := v], s2[x' := v], s2Orig) by {
-              RelState2UpdPreserve(varMapping, s1, s2, s2Orig, x, v);
-            }
-          }
-        case Havoc(vDecls) => 
-          var f := 
-            (vDecl : (var_name, Ty)) => 
-                  if vDecl.0 in varMapping.Keys then (varMapping[vDecl.0], vDecl.1) else vDecl;
-          var vDecls' := Sequences.Map(f, vDecls);
-          
-          calc {
-            WpShallowSimpleCmd(a, Havoc(vDecls), post1)(s1);
-            ForallVarDeclsShallow(a, vDecls, post1)(s1);
-            { ForallVarDeclsRelNew2(a, vDecls, varMapping, post1, post2, s1, s2, s2Orig); }
-            ForallVarDeclsShallow(a, vDecls', post2)(s2);
-            WpShallowSimpleCmd(a, Havoc(vDecls'), post2)(s2);
-            WpShallowSimpleCmd(a, SubstSimpleCmd(Havoc(vDecls), varMapping), post2)(s2);
-          }
-        case SeqSimple(sc1, sc2) =>
-          var sc1' := SubstSimpleCmd(sc1, varMapping);
-          var sc2' := SubstSimpleCmd(sc2, varMapping);
-
-          var post1' := WpShallowSimpleCmd(a, sc2, post1);
-          var post2' := WpShallowSimpleCmd(a, sc2', post2);
-
-
-          calc {
-            WpShallowSimpleCmd(a, SeqSimple(sc1, sc2), post1)(s1);
-            WpShallowSimpleCmd(a, sc1, post1')(s1);
-            { 
-              assert RelPred(varMapping, post1', post2', s2Orig) by {
-                SubstSimpleCmdCorrect(a, sc2, varMapping, post1, post2, s2Orig);
-              }
-              SubstSimpleCmdCorrect(a, sc1, varMapping, post1', post2', s2Orig); 
-            }
-            WpShallowSimpleCmd(a, sc1', post2')(s2);
-            WpShallowSimpleCmd(a, SeqSimple(sc1', sc2'), post2)(s2);
-          }
-      }
-    }
-  }
-
-  predicate {:opaque} RelPost<A(!new)>(m: map<var_name, var_name>, post1: WpPostShallow<A>, post2: WpPostShallow<A>, s2Orig: MapOrig<Val<A>>)
-  {
-    && post1.scopes.Keys == post2.scopes.Keys
-    && RelPred(m, post1.normal, post2.normal, s2Orig)
-    && RelPred(m, post1.currentScope, post2.currentScope, s2Orig)
-    && (forall lbl | lbl in post1.scopes.Keys :: RelPred(m, post1.scopes[lbl], post2.scopes[lbl], s2Orig))
-  }
-
-  lemma ResetVarsStateLookup<A(!new)>(varDecls: seq<VarDecl>, s: state<A>, sOrig: state<A>, x: var_name)
-  requires x in GetVarNames(varDecls)
-  ensures Maps.Get(ResetVarsState(varDecls, s, sOrig), x) == Maps.Get(sOrig, x)
-  { }
-
-  lemma ResetVarsStateLookup2<A(!new)>(varDecls: seq<VarDecl>, s: state<A>, sOrig: state<A>, x: var_name)
-  requires x !in GetVarNames(varDecls)
-  ensures Maps.Get(ResetVarsState(varDecls, s, sOrig), x) == Maps.Get(s, x)
-  { }
-
-  lemma RelStateSwitch<A(!new)>(
-    m: map<var_name, var_name>, 
-    varDecls: seq<VarDecl>, 
-    varDecls': seq<VarDecl>,
-    sA: state<A>, 
-    sB: state<A>, 
-    s1: state<A>,
-    s2: state<A>,
-    s2Orig: MapOrig<Val<A>>)
-  requires |varDecls| == |varDecls'|
-  requires m.Values !! GetVarNames(varDecls')
-  requires s2Orig.Keys !! GetVarNames(varDecls')
-  requires 
-    var s2OrigNewKeys := set x | x in GetVarNames(varDecls) && x in m.Keys :: m[x];
-    var s2Orig' := s2Orig + map x' | x' in s2OrigNewKeys :: Maps.Get(s2, x');
-    var m' := m + ConvertVDeclsToSubstMap(varDecls, varDecls');
-    && RelState2(m', sA, sB, s2Orig')
-    && RelState2(m, s1, s2, s2Orig)
-  requires |varDecls| == |varDecls'|
-  ensures 
-    RelState2(m, ResetVarsState(varDecls, sA, s1), ResetVarsState(varDecls', sB, s2), s2Orig)
+  lemma RelState2UpdPreserve<V>(varMapping: map<var_name, var_name>, s1: map<var_name, V>, s2: map<var_name, V>, s2Orig: MapOrig<V>, x: var_name, v: V)
+  requires RelState2(varMapping, s1, s2, s2Orig)
+  requires Maps.Injective(varMapping)
+  requires x in varMapping.Keys
+  ensures RelState2(varMapping, s1[x := v], s2[varMapping[x] := v], s2Orig)
   {
     reveal RelState2();
-
-    var s2OrigNewKeys := set x | x in GetVarNames(varDecls) && x in m.Keys :: m[x];
-    var s2Orig' := s2Orig + map x' | x' in s2OrigNewKeys :: Maps.Get(s2, x');
-    var mExt := ConvertVDeclsToSubstMap(varDecls, varDecls');
-    var m' := m + mExt;
-
-    var sA' := ResetVarsState(varDecls, sA, s1);
-    var sB' := ResetVarsState(varDecls', sB, s2);
-
-    forall k | k in m.Keys
-    ensures Maps.Get(sA', k) == Maps.Get(sB', m[k])
+    var x' := varMapping[x];
+    forall k | k in varMapping.Keys 
+    ensures Maps.Get(s1[x := v], k) == Maps.Get(s2[varMapping[x] := v], varMapping[k])
     {
-      if k in mExt {
-        assert k in GetVarNames(varDecls);
-        assert m[k] in s2OrigNewKeys;
+      var k' := varMapping[k];
+      if k != x {
         calc {
-          Maps.Get(sB', m[k]);
-          {
-            assert m[k] !in GetVarNames(varDecls');
-            ResetVarsStateLookup2(varDecls', sB, s2, m[k]);
-          }
-          Maps.Get(sB, m[k]);
-          s2Orig'[m[k]];
-          Maps.Get(s2, m[k]);
+          Maps.Get(s1[x := v], k);
           Maps.Get(s1, k);
-          {
-            ResetVarsStateLookup(varDecls, sA, s1, k);
-          }
-          Maps.Get(sA', k);
+          Maps.Get(s2, k');
+          { reveal Maps.Injective(); }
+          Maps.Get(s2[x' := v], k');
         }
-      } else {
-        calc {
-          Maps.Get(sB', m[k]);
-          {
-            assert m[k] !in GetVarNames(varDecls');
-            ResetVarsStateLookup2(varDecls', sB, s2, m[k]);
-          }
-          Maps.Get(sB, m[k]);
-          Maps.Get(sA, k);
-          {
-            assert k !in GetVarNames(varDecls);
-            ResetVarsStateLookup2(varDecls, sA, s1, k);
-          }
-          Maps.Get(sA', k);
-        }
-      }
-    }
-
-    forall k | k in s2Orig.Keys
-    ensures Maps.Get(sB', k) == s2Orig[k]
-    {
-      assert m'.Values !! s2Orig'.Keys;
-      assert m.Values !! s2Orig.Keys;
-      assert m.Values !! GetVarNames(varDecls');
-
-      calc {
-        Maps.Get(sB', k);
-        {
-          assert k !in GetVarNames(varDecls');
-          ResetVarsStateLookup2(varDecls', sB, s2, k);
-        }
-        Maps.Get(sB, k);
-        s2Orig'[k];
-        s2Orig[k];
       }
     }
   }
+
+  lemma RelState2UpdVarDeclsPreserve<A>(
+      varMapping: map<var_name, var_name>, 
+      s1: state<A>,
+      s2: state<A>, 
+      s2Orig: MapOrig<Val<A>>, 
+      varDecls: seq<VarDecl>, 
+      varDecls': seq<VarDecl>,
+      vs: seq<Val<A>>)
+  requires RelState2(varMapping, s1, s2, s2Orig)
+  requires Maps.Injective(varMapping)
+  requires GetVarNames(varDecls) <= varMapping.Keys
+  requires |vs| == |varDecls| == |varDecls'|
+  requires (forall i | 0 <= i < |varDecls| :: varDecls'[i].0 == varMapping[varDecls[i].0])
+  ensures RelState2(varMapping, StateUpdVarDecls(s1, varDecls, vs), StateUpdVarDecls(s2, varDecls', vs), s2Orig)
+  {
+    if |varDecls| > 0 {       
+        var s1' := StateUpdVarDecls(s1, varDecls[1..], vs[1..]);
+        var s2' := StateUpdVarDecls(s2, varDecls'[1..], vs[1..]);
+
+        assert RelState2(varMapping, s1', s2', s2Orig) by {
+          RelState2UpdVarDeclsPreserve(varMapping, s1, s2, s2Orig, varDecls[1..], varDecls'[1..], vs[1..]);
+        }
+
+        RelState2UpdPreserve(varMapping, s1', s2', s2Orig, varDecls[0].0, vs[0]);
+    }
+  }
+
+  lemma ForallVarDeclsRelNew<A(!new)>(
+      a: absval_interp<A>, 
+      varDecls: seq<(var_name, Ty)>, 
+      varMapping: map<var_name, var_name>, 
+      p1: Predicate<A>,
+      p2: Predicate<A>,
+      s2Orig: MapOrig<Val<A>>)
+      requires RelPred(varMapping, p1, p2, s2Orig)
+      requires GetVarNames(varDecls) <= varMapping.Keys
+      requires Maps.Injective(varMapping)
+      ensures 
+        var f := (vDecl : (var_name, Ty)) => 
+            if vDecl.0 in varMapping.Keys then (varMapping[vDecl.0], vDecl.1) else vDecl;
+        var varDecls' := Sequences.Map(f, varDecls);
+        RelPred(varMapping, ForallVarDeclsShallow(a, varDecls, p1), ForallVarDeclsShallow(a, varDecls', p2), s2Orig)
+    {
+      var f := (vDecl : (var_name, Ty)) => 
+          if vDecl.0 in varMapping.Keys then (varMapping[vDecl.0], vDecl.1) else vDecl;
+      var varDecls' := Sequences.Map(f, varDecls);
+      if |varDecls| == 0 {
+        //trivial
+        reveal ForallVarDeclsShallow();
+        assert ForallVarDeclsShallow(a, varDecls, p1) == p1;
+      } else {
+        var (x,t) := varDecls[0];
+        var x' := varMapping[x];
+
+        var f := (vDecl : (var_name, Ty)) => 
+            if vDecl.0 in varMapping.Keys then (varMapping[vDecl.0], vDecl.1) else vDecl;
+        var varDecls' := Sequences.Map(f, varDecls);
+
+        forall s1, s2 | RelState2(varMapping, s1, s2, s2Orig)
+        ensures ForallVarDeclsShallow(a, varDecls, p1)(s1) == ForallVarDeclsShallow(a, varDecls', p2)(s2)
+        {
+          forall vs | ValuesRespectDecls(a, vs, varDecls)
+          ensures p1(StateUpdVarDecls(s1, varDecls, vs)) == p2(StateUpdVarDecls(s2, varDecls', vs))
+          {
+            var s1' := StateUpdVarDecls(s1, varDecls, vs);
+            var s2' := StateUpdVarDecls(s2, varDecls', vs);
+            assert RelState2(varMapping, s1', s2', s2Orig) by {
+              RelState2UpdVarDeclsPreserve(varMapping, s1, s2, s2Orig, varDecls, varDecls', vs);
+            }
+            reveal RelPred();
+          }
+          ForallVarDeclsShallowEquiv(a, varDecls, varDecls', p1, p2, s1, s2);
+        }
+
+        reveal RelPred();
+      }
+    }
+  lemma ForallVarDeclsRelNew2<A(!new)>(
+      a: absval_interp<A>, 
+      varDecls: seq<(var_name, Ty)>, 
+      varMapping: map<var_name, var_name>, 
+      p1: Predicate<A>,
+      p2: Predicate<A>,
+      s1: state<A>,
+      s2: state<A>,
+      sOrig: MapOrig<Val<A>>)
+      requires RelPred(varMapping, p1, p2, sOrig)
+      requires RelState2(varMapping, s1, s2, sOrig)
+      requires GetVarNames(varDecls) <= varMapping.Keys
+      requires Maps.Injective(varMapping)
+      ensures 
+        var f := (vDecl : (var_name, Ty)) => 
+            if vDecl.0 in varMapping.Keys then (varMapping[vDecl.0], vDecl.1) else vDecl;
+        var varDecls' := Sequences.Map(f, varDecls);
+        ForallVarDeclsShallow(a, varDecls, p1)(s1) ==  ForallVarDeclsShallow(a, varDecls', p2)(s2)
+    {
+      ForallVarDeclsRelNew(a, varDecls, varMapping, p1, p2, sOrig);
+      reveal RelPred();
+    }
+
+  lemma {:induction false} SubstSimpleCmdCorrect<A(!new)>(a: absval_interp<A>, sc: SimpleCmd, varMapping: map<var_name, var_name>, 
+      post1: Predicate<A>, post2: Predicate<A>, s2Orig: MapOrig<Val<A>>)
+      requires RelPred(varMapping, post1, post2, s2Orig)
+      requires sc.WellFormedVars(varMapping.Keys)
+      requires Maps.Injective(varMapping)
+      ensures 
+        var sc' := SubstSimpleCmd(sc, varMapping);
+        RelPred(varMapping, WpShallowSimpleCmd(a, sc, post1), WpShallowSimpleCmd(a, sc', post2), s2Orig)
+    {
+      var sc' := SubstSimpleCmd(sc, varMapping);
+      var pre1 := WpShallowSimpleCmd(a, sc, post1);
+      var pre2 := WpShallowSimpleCmd(a, sc', post2);
+      forall s1:map<var_name, Val<A>>, s2 | RelState2(varMapping, s1, s2, s2Orig)
+        ensures pre1(s1) == pre2(s2)
+      {
+        reveal RelPred();
+        match sc {
+          case Skip => 
+          case Assume(e) => 
+            reveal RelState2();
+            MultiSubstExprSpec2(a, varMapping, e, s1, s2);
+          case Assert(e) => 
+            reveal RelState2();
+            reveal RelPred();
+            MultiSubstExprSpec2(a, varMapping, e, s1, s2);
+          case Assign(x, t, e) =>
+            var e' := MultiSubstExpr(e, varMapping);
+            var v1Opt := EvalExpr(a, e, s1);
+            var v2Opt := EvalExpr(a, e', s2);
+            assert v1Opt == v2Opt by {
+              reveal RelState2();
+              MultiSubstExprSpec2(a, varMapping, e, s1, s2);
+            }
+
+            if(v1Opt.Some?) {
+              var v := v1Opt.value;
+              var x' := varMapping[x];
+
+              assert RelState2(varMapping, s1[x := v], s2[x' := v], s2Orig) by {
+                RelState2UpdPreserve(varMapping, s1, s2, s2Orig, x, v);
+              }
+            }
+          case Havoc(vDecls) => 
+            var f := 
+              (vDecl : (var_name, Ty)) => 
+                    if vDecl.0 in varMapping.Keys then (varMapping[vDecl.0], vDecl.1) else vDecl;
+            var vDecls' := Sequences.Map(f, vDecls);
+            
+            calc {
+              WpShallowSimpleCmd(a, Havoc(vDecls), post1)(s1);
+              ForallVarDeclsShallow(a, vDecls, post1)(s1);
+              { ForallVarDeclsRelNew2(a, vDecls, varMapping, post1, post2, s1, s2, s2Orig); }
+              ForallVarDeclsShallow(a, vDecls', post2)(s2);
+              WpShallowSimpleCmd(a, Havoc(vDecls'), post2)(s2);
+              WpShallowSimpleCmd(a, SubstSimpleCmd(Havoc(vDecls), varMapping), post2)(s2);
+            }
+          case SeqSimple(sc1, sc2) =>
+            var sc1' := SubstSimpleCmd(sc1, varMapping);
+            var sc2' := SubstSimpleCmd(sc2, varMapping);
+
+            var post1' := WpShallowSimpleCmd(a, sc2, post1);
+            var post2' := WpShallowSimpleCmd(a, sc2', post2);
+
+
+            calc {
+              WpShallowSimpleCmd(a, SeqSimple(sc1, sc2), post1)(s1);
+              WpShallowSimpleCmd(a, sc1, post1')(s1);
+              { 
+                assert RelPred(varMapping, post1', post2', s2Orig) by {
+                  SubstSimpleCmdCorrect(a, sc2, varMapping, post1, post2, s2Orig);
+                }
+                SubstSimpleCmdCorrect(a, sc1, varMapping, post1', post2', s2Orig); 
+              }
+              WpShallowSimpleCmd(a, sc1', post2')(s2);
+              WpShallowSimpleCmd(a, SeqSimple(sc1', sc2'), post2)(s2);
+            }
+        }
+      }
+    }
+
+    predicate {:opaque} RelPost<A(!new)>(m: map<var_name, var_name>, post1: WpPostShallow<A>, post2: WpPostShallow<A>, s2Orig: MapOrig<Val<A>>)
+    {
+      && post1.scopes.Keys == post2.scopes.Keys
+      && RelPred(m, post1.normal, post2.normal, s2Orig)
+      && RelPred(m, post1.currentScope, post2.currentScope, s2Orig)
+      && (forall lbl | lbl in post1.scopes.Keys :: RelPred(m, post1.scopes[lbl], post2.scopes[lbl], s2Orig))
+    }
+
+    lemma ResetVarsStateLookup<A(!new)>(varDecls: seq<VarDecl>, s: state<A>, sOrig: state<A>, x: var_name)
+    requires x in GetVarNames(varDecls)
+    ensures Maps.Get(ResetVarsState(varDecls, s, sOrig), x) == Maps.Get(sOrig, x)
+    { }
+
+    lemma ResetVarsStateLookup2<A(!new)>(varDecls: seq<VarDecl>, s: state<A>, sOrig: state<A>, x: var_name)
+    requires x !in GetVarNames(varDecls)
+    ensures Maps.Get(ResetVarsState(varDecls, s, sOrig), x) == Maps.Get(s, x)
+    { }
+
+    lemma RelStateSwitch<A(!new)>(
+      m: map<var_name, var_name>, 
+      varDecls: seq<VarDecl>, 
+      varDecls': seq<VarDecl>,
+      sA: state<A>, 
+      sB: state<A>, 
+      s1: state<A>,
+      s2: state<A>,
+      s2Orig: MapOrig<Val<A>>)
+    requires |varDecls| == |varDecls'|
+    requires m.Values !! GetVarNames(varDecls')
+    requires s2Orig.Keys !! GetVarNames(varDecls')
+    requires 
+      var s2OrigNewKeys := set x | x in GetVarNames(varDecls) && x in m.Keys :: m[x];
+      var s2Orig' := s2Orig + map x' | x' in s2OrigNewKeys :: Maps.Get(s2, x');
+      var m' := m + ConvertVDeclsToSubstMap(varDecls, varDecls');
+      && RelState2(m', sA, sB, s2Orig')
+      && RelState2(m, s1, s2, s2Orig)
+    requires |varDecls| == |varDecls'|
+    ensures 
+      RelState2(m, ResetVarsState(varDecls, sA, s1), ResetVarsState(varDecls', sB, s2), s2Orig)
+    {
+      reveal RelState2();
+
+      var s2OrigNewKeys := set x | x in GetVarNames(varDecls) && x in m.Keys :: m[x];
+      var s2Orig' := s2Orig + map x' | x' in s2OrigNewKeys :: Maps.Get(s2, x');
+      var mExt := ConvertVDeclsToSubstMap(varDecls, varDecls');
+      var m' := m + mExt;
+
+      var sA' := ResetVarsState(varDecls, sA, s1);
+      var sB' := ResetVarsState(varDecls', sB, s2);
+
+      forall k | k in m.Keys
+      ensures Maps.Get(sA', k) == Maps.Get(sB', m[k])
+      {
+        if k in mExt {
+          assert k in GetVarNames(varDecls);
+          assert m[k] in s2OrigNewKeys;
+          calc {
+            Maps.Get(sB', m[k]);
+            {
+              assert m[k] !in GetVarNames(varDecls');
+              ResetVarsStateLookup2(varDecls', sB, s2, m[k]);
+            }
+            Maps.Get(sB, m[k]);
+            s2Orig'[m[k]];
+            Maps.Get(s2, m[k]);
+            Maps.Get(s1, k);
+            {
+              ResetVarsStateLookup(varDecls, sA, s1, k);
+            }
+            Maps.Get(sA', k);
+          }
+        } else {
+          calc {
+            Maps.Get(sB', m[k]);
+            {
+              assert m[k] !in GetVarNames(varDecls');
+              ResetVarsStateLookup2(varDecls', sB, s2, m[k]);
+            }
+            Maps.Get(sB, m[k]);
+            Maps.Get(sA, k);
+            {
+              assert k !in GetVarNames(varDecls);
+              ResetVarsStateLookup2(varDecls, sA, s1, k);
+            }
+            Maps.Get(sA', k);
+          }
+        }
+      }
+
+      forall k | k in s2Orig.Keys
+      ensures Maps.Get(sB', k) == s2Orig[k]
+      {
+        assert m'.Values !! s2Orig'.Keys;
+        assert m.Values !! s2Orig.Keys;
+        assert m.Values !! GetVarNames(varDecls');
+
+        calc {
+          Maps.Get(sB', k);
+          {
+            assert k !in GetVarNames(varDecls');
+            ResetVarsStateLookup2(varDecls', sB, s2, k);
+          }
+          Maps.Get(sB, k);
+          s2Orig'[k];
+          s2Orig[k];
+        }
+      }
+    }
 
   lemma RelPredSwitch<A(!new)>(
     m: map<var_name, var_name>, 
@@ -710,236 +688,200 @@ module DesugarScopedVarsProof {
     } 
 
 
- lemma {:induction false} DesugarScopedVarsCorrect<A(!new)>(
-      a: absval_interp<A>,
-      c: Cmd, 
-      substMap: map<var_name, var_name>, 
-      counter: nat,
-      post1: WpPostShallow<A>,
-      post2: WpPostShallow<A>,
-      s2Orig: MapOrig<Val<A>>,
-      names: set<string>)
-    requires c.WellFormedVars(substMap.Keys)
-    requires Maps.Injective(substMap)
-    requires 
-      var (c', counter') := DesugarScopedVars(c, substMap, counter);
-      && LabelsWellDefAux(c, post1.scopes.Keys) 
-      && LabelsWellDefAux(c', post2.scopes.Keys)
-      && RelPost(substMap, post1, post2, s2Orig)
-      && s2Orig.Keys <= VarNameSet(names, 0, counter)
-      && substMap.Values <= VarNameSet(names, 0, counter) 
-    //requires forall vDecl | vDecls in seqSubstMap :: substMap(vDecl.) == sequSubstMap
-    ensures 
-      var (c', counter') := DesugarScopedVars(c, substMap, counter);
-      RelPred(substMap, WpShallow(a, c, post1), WpShallow(a, c', post2), s2Orig)
-    /** proof sketch notes:  
-      for scopes case, will have to show that the updated substMap remains injective 
-    */
-  {
-    reveal RelPost();
-    match c {
-      case SimpleCmd(sc) =>
-        reveal WpShallow();
-        SubstSimpleCmdCorrect(a, sc, substMap, post1.normal, post2.normal, s2Orig);
-      case Break(_) => reveal WpShallow();
-      case Seq(c1, c2) => 
-        var (c1', counter1') := DesugarScopedVars(c1, substMap, counter);
-        var (c2', counter2') := DesugarScopedVars(c2, substMap, counter1');
+  lemma {:induction false} DesugarScopedVarsCorrect<A(!new)>(
+        a: absval_interp<A>,
+        c: Cmd, 
+        substMap: map<var_name, var_name>, 
+        counter: nat,
+        post1: WpPostShallow<A>,
+        post2: WpPostShallow<A>,
+        s2Orig: MapOrig<Val<A>>,
+        names: set<string>)
+      requires c.WellFormedVars(substMap.Keys)
+      requires Maps.Injective(substMap)
+      requires 
+        var (c', counter') := DesugarScopedVars(c, substMap, counter);
+        && LabelsWellDefAux(c, post1.scopes.Keys) 
+        && LabelsWellDefAux(c', post2.scopes.Keys)
+        && RelPost(substMap, post1, post2, s2Orig)
+        && s2Orig.Keys <= VarNameSet(names, 0, counter)
+        && substMap.Values <= VarNameSet(names, 0, counter) 
+      //requires forall vDecl | vDecls in seqSubstMap :: substMap(vDecl.) == sequSubstMap
+      ensures 
+        var (c', counter') := DesugarScopedVars(c, substMap, counter);
+        RelPred(substMap, WpShallow(a, c, post1), WpShallow(a, c', post2), s2Orig)
+      /** proof sketch notes:  
+        for scopes case, will have to show that the updated substMap remains injective 
+      */
+    {
+      reveal RelPost();
+      match c {
+        case SimpleCmd(sc) =>
+          reveal WpShallow();
+          SubstSimpleCmdCorrect(a, sc, substMap, post1.normal, post2.normal, s2Orig);
+        case Break(_) => reveal WpShallow();
+        case Seq(c1, c2) => 
+          var (c1', counter1') := DesugarScopedVars(c1, substMap, counter);
+          var (c2', counter2') := DesugarScopedVars(c2, substMap, counter1');
 
-        var post1' := WpPostShallow(WpShallow(a, c2, post1), post1.currentScope, post1.scopes);
-        var post2' := WpPostShallow(WpShallow(a, c2', post2), post2.currentScope, post2.scopes);
+          var post1' := WpPostShallow(WpShallow(a, c2, post1), post1.currentScope, post1.scopes);
+          var post2' := WpPostShallow(WpShallow(a, c2', post2), post2.currentScope, post2.scopes);
 
-        assert RelPost(substMap, post1', post2', s2Orig) by {
-          assert RelPred(substMap, WpShallow(a, c2, post1), WpShallow(a, c2', post2), s2Orig) by {
-            VarNameSetExtend(names, 0, counter, counter1');
-            DesugarScopedVarsCorrect(a, c2, substMap, counter1', post1, post2, s2Orig, names);
-          }
-        }
-
-        assert RelPred(substMap, WpShallow(a, c1, post1'), WpShallow(a, c1', post2'), s2Orig) by {
-          DesugarScopedVarsCorrect(a, c1, substMap, counter, post1', post2', s2Orig, names);
-        }
-
-        reveal WpShallow();
-      case Scope(optLabel, varDecls, body) => 
-        /* Goal: RelPred(substMap, WpShallow(a, c, post1), WpShallow(a, c', post2)) */
-        var varDecls' := CreateUniqueVarDecls(varDecls, counter);
-
-        assert Sequences.HasNoDuplicates(GetVarNamesSeq(varDecls')) by {
-          CreateUniqueVarDeclsNoDup(varDecls, counter);
-        }
-
-        var counter' := counter + |varDecls'|;
-        var substMap' := substMap + ConvertVDeclsToSubstMap(varDecls, varDecls');
-        assert substMap'.Keys == GetVarNames(varDecls)+substMap.Keys;
-        var (body', counter'') := DesugarScopedVars(body, substMap', counter');
-        //(Scope(optLabel, varDecls', body''), counter'')
-        var c' := Scope(optLabel, varDecls', body');
-
-        var updatedScopes1 := 
-          if optLabel.Some? then 
-            post1.scopes[optLabel.value := post1.normal]
-          else post1.scopes;
-        assert updatedScopes1.Keys == if optLabel.Some? then {optLabel.value} + post1.scopes.Keys else post1.scopes.Keys;
-        
-        var updatedScopes2 := 
-          if optLabel.Some? then 
-            post2.scopes[optLabel.value := post2.normal]
-          else post2.scopes;
-        assert updatedScopes2.Keys == if optLabel.Some? then {optLabel.value} + post2.scopes.Keys else post2.scopes.Keys;
-        
-        var post1' := WpPostShallow(post1.normal, post1.normal, updatedScopes1);
-        var post2' := WpPostShallow(post2.normal, post2.normal, updatedScopes2);
-
-        forall s1,s2 | RelState2(substMap, s1, s2, s2Orig)
-        ensures WpShallow(a, c, post1)(s1) == WpShallow(a, c', post2)(s2)
-        {
-          /* We want to prove that if a name x in varDecls is already mapped to x' in substMap, then 
-            it must be the case that x' will not be modified within the scope, since we map x to a new
-            name and x' won't be reused in the scope. We need this to make sure that when the scope is finished
-            and the variables are reset, x and x' are again related in the resulting states (
-              for x we know the value is reset to the previous value, for x' we prove the value cannot have changed
-            ). */
-          var s2OrigNewKeys := set x | x in GetVarNames(varDecls) && x in substMap.Keys :: substMap[x];
-          var s2Orig' := s2Orig + map x' | x' in s2OrigNewKeys :: Maps.Get(s2, x');
-
-          assert 
-            && substMap.Values !! GetVarNames(varDecls')
-            && s2Orig.Keys !! GetVarNames(varDecls') by {
-            VarNameSetDisjoint(names, GetVarNames(varDecls), 0, counter, counter, counter + |varDecls'|);
-          }
-
-          calc {
-            WpShallow(a, Scope(optLabel, varDecls, body), post1)(s1);
-            {reveal WpShallow();}
-            ForallVarDeclsShallow(a, varDecls, WpShallow(a, body, ResetVarsPost(varDecls, post1', s1)))(s1);
-            { 
-              assert RelPost(substMap', ResetVarsPost(varDecls, post1', s1), ResetVarsPost(varDecls', post2', s2), s2Orig') by 
-              { 
-                assert RelPost(substMap, post1, post2, s2Orig);
-
-                assert RelPost(substMap, post1', post2', s2Orig);
-                {
-                  reveal RelPost();
-                }
-
-                RelPostSwitch(substMap, varDecls, varDecls', post1', post2', s1, s2, s2Orig);
-              }
-
-              assert Maps.Injective(substMap') by {
-                assert Maps.Injective(ConvertVDeclsToSubstMap(varDecls, varDecls')) by {
-                  ConvertVDeclsToSubstMapInj(varDecls, varDecls');
-                }
-                assert substMap.Values !! GetVarNames(varDecls');
-                UnionOfInjectiveMaps(substMap, ConvertVDeclsToSubstMap(varDecls, varDecls'));
-              }
-
-              assert RelPred(substMap', 
-                WpShallow(a, body, ResetVarsPost(varDecls, post1', s1)), 
-                WpShallow(a, body', ResetVarsPost(varDecls', post2', s2)),
-                s2Orig') by
-                { 
-                  assert s2Orig'.Keys <= VarNameSet(names+GetVarNames(varDecls), 0, counter') by {
-                    VarNameSetExtend2(names, GetVarNames(varDecls), 0, counter, counter');
-                  }
-
-                  assert substMap'.Values <= VarNameSet(names+GetVarNames(varDecls), 0, counter') by {
-                    assert substMap'.Values <= VarNameSet(names, 0, counter) + VarNameSet(GetVarNames(varDecls), counter, counter + |varDecls|);
-                    VarNameSetAppend(names, GetVarNames(varDecls), 0, counter, counter, counter + |varDecls|);
-                  }
-
-                  DesugarScopedVarsCorrect(
-                    a, body, substMap', counter',  ResetVarsPost(varDecls, post1', s1), ResetVarsPost(varDecls', post2', s2), s2Orig',
-                    names+GetVarNames(varDecls)
-                  ); 
-                }
-                
-                var p1 := WpShallow(a, body, ResetVarsPost(varDecls, post1', s1));
-                var p2 := WpShallow(a, body', ResetVarsPost(varDecls', post2', s2));
-
-                ForallVarDeclsRelSwitch(
-                    a, 
-                    varDecls, 
-                    varDecls',
-                    substMap, 
-                    p1,
-                    p2,
-                    s1,
-                    s2,
-                    s2Orig);
+          assert RelPost(substMap, post1', post2', s2Orig) by {
+            assert RelPred(substMap, WpShallow(a, c2, post1), WpShallow(a, c2', post2), s2Orig) by {
+              VarNameSetExtend(names, 0, counter, counter1');
+              DesugarScopedVarsCorrect(a, c2, substMap, counter1', post1, post2, s2Orig, names);
             }
-            ForallVarDeclsShallow(a, varDecls', WpShallow(a, body', ResetVarsPost(varDecls', post2', s2)))(s2);
-            {reveal WpShallow();}
-            WpShallow(a, Scope(optLabel, varDecls', body'), post2)(s2);
           }
-        }
 
-        reveal RelPred();
-      case If(None, thn, els) => 
-        var (thn', counter') := DesugarScopedVars(thn, substMap, counter);
-        var (els', counter'') := DesugarScopedVars(els, substMap, counter');
-
-        assert RelPred(substMap, WpShallow(a, thn, post1), WpShallow(a, thn', post2), s2Orig) by {
-          DesugarScopedVarsCorrect(a, thn, substMap, counter, post1, post2, s2Orig, names);
-        }
-
-        assert RelPred(substMap, WpShallow(a, els, post1), WpShallow(a, els', post2), s2Orig) by {
-          VarNameSetExtend(names, 0, counter, counter');
-          DesugarScopedVarsCorrect(a, els, substMap, counter', post1, post2, s2Orig, names);
-        }
-
-        reveal RelPred();
-
-        forall sA, sB | RelState2(substMap, sA, sB, s2Orig)
-        ensures WpShallow(a, c, post1)(sA) == WpShallow(a, If(None, thn', els'), post2)(sB)
-        {
-          calc {
-            WpShallow(a, c, post1)(sA);
-            { reveal WpShallow(); }
-            Util.AndOpt(WpShallow(a, thn, post1)(sA), WpShallow(a, els, post1)(sA));
-            Util.AndOpt(WpShallow(a, thn', post2)(sB), WpShallow(a, els', post2)(sB));
-            { reveal WpShallow(); }
-            WpShallow(a, If(None, thn', els'), post2)(sB);
+          assert RelPred(substMap, WpShallow(a, c1, post1'), WpShallow(a, c1', post2'), s2Orig) by {
+            DesugarScopedVarsCorrect(a, c1, substMap, counter, post1', post2', s2Orig, names);
           }
-        }
-      case _ => assume false;
+
+          reveal WpShallow();
+        case Scope(optLabel, varDecls, body) => 
+          /* Goal: RelPred(substMap, WpShallow(a, c, post1), WpShallow(a, c', post2)) */
+          var varDecls' := CreateUniqueVarDecls(varDecls, counter);
+
+          assert Sequences.HasNoDuplicates(GetVarNamesSeq(varDecls')) by {
+            CreateUniqueVarDeclsNoDup(varDecls, counter);
+          }
+
+          var counter' := counter + |varDecls'|;
+          var substMap' := substMap + ConvertVDeclsToSubstMap(varDecls, varDecls');
+          assert substMap'.Keys == GetVarNames(varDecls)+substMap.Keys;
+          var (body', counter'') := DesugarScopedVars(body, substMap', counter');
+          //(Scope(optLabel, varDecls', body''), counter'')
+          var c' := Scope(optLabel, varDecls', body');
+
+          var updatedScopes1 := 
+            if optLabel.Some? then 
+              post1.scopes[optLabel.value := post1.normal]
+            else post1.scopes;
+          assert updatedScopes1.Keys == if optLabel.Some? then {optLabel.value} + post1.scopes.Keys else post1.scopes.Keys;
+          
+          var updatedScopes2 := 
+            if optLabel.Some? then 
+              post2.scopes[optLabel.value := post2.normal]
+            else post2.scopes;
+          assert updatedScopes2.Keys == if optLabel.Some? then {optLabel.value} + post2.scopes.Keys else post2.scopes.Keys;
+          
+          var post1' := WpPostShallow(post1.normal, post1.normal, updatedScopes1);
+          var post2' := WpPostShallow(post2.normal, post2.normal, updatedScopes2);
+
+          forall s1,s2 | RelState2(substMap, s1, s2, s2Orig)
+          ensures WpShallow(a, c, post1)(s1) == WpShallow(a, c', post2)(s2)
+          {
+            /* We want to prove that if a name x in varDecls is already mapped to x' in substMap, then 
+              it must be the case that x' will not be modified within the scope, since we map x to a new
+              name and x' won't be reused in the scope. We need this to make sure that when the scope is finished
+              and the variables are reset, x and x' are again related in the resulting states (
+                for x we know the value is reset to the previous value, for x' we prove the value cannot have changed
+              ). */
+            var s2OrigNewKeys := set x | x in GetVarNames(varDecls) && x in substMap.Keys :: substMap[x];
+            var s2Orig' := s2Orig + map x' | x' in s2OrigNewKeys :: Maps.Get(s2, x');
+
+            assert 
+              && substMap.Values !! GetVarNames(varDecls')
+              && s2Orig.Keys !! GetVarNames(varDecls') by {
+              VarNameSetDisjoint(names, GetVarNames(varDecls), 0, counter, counter, counter + |varDecls'|);
+            }
+
+            calc {
+              WpShallow(a, Scope(optLabel, varDecls, body), post1)(s1);
+              {reveal WpShallow();}
+              ForallVarDeclsShallow(a, varDecls, WpShallow(a, body, ResetVarsPost(varDecls, post1', s1)))(s1);
+              { 
+                assert RelPost(substMap', ResetVarsPost(varDecls, post1', s1), ResetVarsPost(varDecls', post2', s2), s2Orig') by 
+                { 
+                  assert RelPost(substMap, post1, post2, s2Orig);
+
+                  assert RelPost(substMap, post1', post2', s2Orig);
+                  {
+                    reveal RelPost();
+                  }
+
+                  RelPostSwitch(substMap, varDecls, varDecls', post1', post2', s1, s2, s2Orig);
+                }
+
+                assert Maps.Injective(substMap') by {
+                  assert Maps.Injective(ConvertVDeclsToSubstMap(varDecls, varDecls')) by {
+                    ConvertVDeclsToSubstMapInj(varDecls, varDecls');
+                  }
+                  assert substMap.Values !! GetVarNames(varDecls');
+                  UnionOfInjectiveMaps(substMap, ConvertVDeclsToSubstMap(varDecls, varDecls'));
+                }
+
+                assert RelPred(substMap', 
+                  WpShallow(a, body, ResetVarsPost(varDecls, post1', s1)), 
+                  WpShallow(a, body', ResetVarsPost(varDecls', post2', s2)),
+                  s2Orig') by
+                  { 
+                    assert s2Orig'.Keys <= VarNameSet(names+GetVarNames(varDecls), 0, counter') by {
+                      VarNameSetExtend2(names, GetVarNames(varDecls), 0, counter, counter');
+                    }
+
+                    assert substMap'.Values <= VarNameSet(names+GetVarNames(varDecls), 0, counter') by {
+                      assert substMap'.Values <= VarNameSet(names, 0, counter) + VarNameSet(GetVarNames(varDecls), counter, counter + |varDecls|);
+                      VarNameSetAppend(names, GetVarNames(varDecls), 0, counter, counter, counter + |varDecls|);
+                    }
+
+                    DesugarScopedVarsCorrect(
+                      a, body, substMap', counter',  ResetVarsPost(varDecls, post1', s1), ResetVarsPost(varDecls', post2', s2), s2Orig',
+                      names+GetVarNames(varDecls)
+                    ); 
+                  }
+                  
+                  var p1 := WpShallow(a, body, ResetVarsPost(varDecls, post1', s1));
+                  var p2 := WpShallow(a, body', ResetVarsPost(varDecls', post2', s2));
+
+                  ForallVarDeclsRelSwitch(
+                      a, 
+                      varDecls, 
+                      varDecls',
+                      substMap, 
+                      p1,
+                      p2,
+                      s1,
+                      s2,
+                      s2Orig);
+              }
+              ForallVarDeclsShallow(a, varDecls', WpShallow(a, body', ResetVarsPost(varDecls', post2', s2)))(s2);
+              {reveal WpShallow();}
+              WpShallow(a, Scope(optLabel, varDecls', body'), post2)(s2);
+            }
+          }
+
+          reveal RelPred();
+        case If(None, thn, els) => 
+          var (thn', counter') := DesugarScopedVars(thn, substMap, counter);
+          var (els', counter'') := DesugarScopedVars(els, substMap, counter');
+
+          assert RelPred(substMap, WpShallow(a, thn, post1), WpShallow(a, thn', post2), s2Orig) by {
+            DesugarScopedVarsCorrect(a, thn, substMap, counter, post1, post2, s2Orig, names);
+          }
+
+          assert RelPred(substMap, WpShallow(a, els, post1), WpShallow(a, els', post2), s2Orig) by {
+            VarNameSetExtend(names, 0, counter, counter');
+            DesugarScopedVarsCorrect(a, els, substMap, counter', post1, post2, s2Orig, names);
+          }
+
+          reveal RelPred();
+
+          forall sA, sB | RelState2(substMap, sA, sB, s2Orig)
+          ensures WpShallow(a, c, post1)(sA) == WpShallow(a, If(None, thn', els'), post2)(sB)
+          {
+            calc {
+              WpShallow(a, c, post1)(sA);
+              { reveal WpShallow(); }
+              Util.AndOpt(WpShallow(a, thn, post1)(sA), WpShallow(a, els, post1)(sA));
+              Util.AndOpt(WpShallow(a, thn', post2)(sB), WpShallow(a, els', post2)(sB));
+              { reveal WpShallow(); }
+              WpShallow(a, If(None, thn', els'), post2)(sB);
+            }
+          }
+        case _ => assume false;
+      }
     }
-  }
-
-function method RemoveScopedVars(c: Cmd): (Cmd, (seq<(var_name, Ty)>))
-  /*requires substMap.Values <= set c,x | x in substMap.Keys && 0 < c < usedVars.1 :: VersionedName(x, c)
-  requires forall x | x in substMap.Keys :: exists c : nat :: c <= usedVars.1 && substMap[x] == VersionedName(x, c)
-  ensures 
-    forall x | x in substMap.Keys :: exists c : nat :: c <= usedVars.1 && substMap[x] == VersionedName(x, c)*/
-{
-  match c
-  case SimpleCmd(sc) => (c, [])
-  case Break(_) => (c, [])
-  case Seq(c1, c2) => 
-    var (c1', decls1) := RemoveScopedVars(c1);
-    var (c2', decls2) := RemoveScopedVars(c2);
-    (Seq(c1', c2'), decls1 + decls2)
-  case Scope(optLabel, varDecls, body) =>
-    var (body', declsBody) := RemoveScopedVars(body);
-    (Scope(optLabel, [], body'), varDecls + declsBody)
-  case If(None, thn, els) => 
-    //TODO: make sure If(Some(...)) has been desugared
-    var (thn', declsThn) := RemoveScopedVars(thn);
-    var (els', declsEls) := RemoveScopedVars(els);
-    (If(None, thn', els'), declsThn + declsEls)
-  case _ => (c, []) //TODO (precondition should eliminate this case)
-}
-
-lemma RelStateRemoveScopedVarsCorrect<A(!new)>(a: absval_interp<A>, c: Cmd, post: WpPostShallow<A>)
-  requires 
-    var (c', decls) := RemoveScopedVars(c);
-    LabelsWellDefAux(c, post.scopes.Keys) && LabelsWellDefAux(c', post.scopes.Keys)
-  ensures 
-    var (c', decls) := RemoveScopedVars(c);
-    forall s :: WpShallow(a, c, post)(s) == ForallVarDeclsShallow(a, decls, WpShallow(a, c', ResetVarsPost(decls, post, s)))(s)
-  /* almost the same as Scope(None, decls, body)
-     Main difference is that currentScope is not updated.
-     If show that body has no direct breaks, then it would be the same
-  */
 
 }
