RemoveScopedVarsProof.dfy
@@ -1,0 +1,29 @@
+include "BoogieSemantics.dfy"
+include "DesugarScopedVarsImpl.dfy"
+include "Naming.dfy"
+include "dafny-libraries/src/Collections/Sequences/Seq.dfy"
+include "dafny-libraries/src/Collections/Maps/Maps.dfy"
+
+module DesugarScopedVarsProof {
+
+  import opened BoogieLang
+  import opened BoogieSemantics
+  import Sequences = Seq
+  import Maps
+  import Util
+  import opened Wrappers
+  import opened DesugarScopedVarsImpl
+  import opened Naming
+
+  lemma RelStateRemoveScopedVarsCorrect<A(!new)>(a: absval_interp<A>, c: Cmd, post: WpPostShallow<A>)
+    requires 
+      var (c', decls) := RemoveScopedVars(c);
+      LabelsWellDefAux(c, post.scopes.Keys) && LabelsWellDefAux(c', post.scopes.Keys)
+    ensures 
+      var (c', decls) := RemoveScopedVars(c);
+      forall s :: WpShallow(a, c, post)(s) == ForallVarDeclsShallow(a, decls, WpShallow(a, c', ResetVarsPost(decls, post, s)))(s)
+    /* almost the same as Scope(None, decls, body)
+      Main difference is that currentScope is not updated.
+      If show that body has no direct breaks, then it would be the same
+    */
+}
